DigitalObjects/TxLib.lean
@@ -1,2 +1,3 @@
 import DigitalObjects.TxLib.Events
 import DigitalObjects.TxLib.Predicates
+import DigitalObjects.TxLib.PredicatesSimple
